Isomorphism trees-fixpoint of container

examples/BTree.v
@@ -12,6 +12,13 @@ Require Import HYLO.Hylo.
 
 Require List.
 
+Tactic Notation "|{" ident(x)  "~>" uconstr(T) "}|" :=
+  refine {| app := fun x => T |};
+  try (intros ??->; reflexivity);
+  try (let H := fresh "H" in intros ?? H; simpl in H; subst; reflexivity);
+  try (intros [??] [??] [E1 E2]; simpl in *;  subst; auto with ffix).
+
+
 (* Defining a tree *)
 Unset Auto Template Polymorphism.
 
@@ -24,13 +31,11 @@ Inductive Ts L A := | Leaf (ELEM : L) | Node (ELEM : A).
 Inductive Tp := | Lbranch | Rbranch. (* positions *)
 (* position valid in shape? *)
 Definition t_dom {L A} : Ts L A * Tp ~> bool.
-  refine {| app := fun x =>
-                     match x with
-                     | (Node _ _, _)  => true
-                     | _            => false
-                     end
-         |}.
-  intros [??] [??] [E1 E2]. simpl in *.  subst. auto.
+|{ x ~> match x with
+     | (Node _ _, _)  => true
+     | _            => false
+     end
+  }|.
 Defined.
 #[local]
   Instance TreeF (L A : Type) : Cont (Ts L A) Tp :=
@@ -62,20 +67,77 @@ Notation leftB  := (e_lbranch eq_refl).
 Notation rightB := (e_rbranch eq_refl).
 
 Definition a_out {L A X : Type} : App (TreeF L A) X ~> ITreeF L A X.
-    refine
-      {| app :=
-          fun x : App (TreeF L A) X =>
-            let (s, k) := x in
-            match s as s' return s = s' -> ITreeF L A X with
-            | Leaf _ x => fun _ => leaf x
-            | Node _ n => fun E => node n (k (e_lbranch E)) (k (e_rbranch E))
-            end eq_refl
-      |}.
+  refine {|
+      app := fun (x : App (TreeF L A) X) =>
+               let (s, k) := x in
+               match s as s' return s = s' -> ITreeF L A X with
+               | Leaf _ x => fun _ => leaf x
+               | Node _ n => fun E => node n (k (e_lbranch E)) (k (e_rbranch E))
+               end eq_refl
+    |}.
   intros [x Fx] [y Fy] [Sxy Kxy]. simpl in *. subst.
   destruct y; trivial; simpl.
   rewrite (Kxy leftB leftB); trivial.
   rewrite (Kxy rightB rightB); trivial.
 Defined.
+
+Inductive itree L A := | i_leaf (l : L) | i_node (x : A) (l r : itree L A).
+Definition to_tree {L A} : itree L A ~> App (TreeF L A) (itree L A).
+|{ x ~>
+     match x with
+     | i_leaf _ l => a_leaf l
+     | i_node n l r => a_node n l r
+     end
+  }|.
+Defined.
+
+Lemma to_tree_rec {L A} : RecP (@to_tree L A).
+Proof.
+  intros x. induction x as [l|n l Ihl r Ihr]; constructor; simpl; intros e.
+  - apply (dom_leaf _ e).
+  - destruct (val e); trivial.
+Defined.
+
+Definition fto_tree {L A}: RCoalg (TreeF L A) (itree L A) := Rec to_tree_rec.
+
+Definition itree_to_tree {L A} : itree L A ~> Tree L A :=
+  rana fto_tree.
+
+Definition to_itree {L A} : App (TreeF L A) (itree L A) ~> itree L A.
+|{ x ~>
+     match a_out x with
+     | leaf l => i_leaf _ l
+     | node n l r => i_node n l r
+     end
+  }|.
+Defined.
+Definition tree_to_itree {L A} : Tree L A ~> itree L A
+  := cata to_itree.
+
+Lemma tree_itree_iso1 {L A} : itree_to_tree (L:=L) (A:=A) \o tree_to_itree =e id.
+  Opaque to_tree_rec.
+  Opaque cata.
+  Opaque rana.
+  intros x. unfold tree_to_itree, itree_to_tree.
+  induction x as [[[|n] kx] Ih]; rewrite cata_unfold, rana_unfold; simpl in *.
+  - split; trivial. intros e. apply (dom_leaf _ e).
+  - split; trivial. intros [[|] V1] [v2 V2]; simpl.
+    + intros <-. rewrite elem_val_eq with (e1:=leftB) (e2:= {|val := Lbranch; Valid := V2|}); trivial.
+    + intros <-. rewrite elem_val_eq with (e1:=rightB) (e2:= {|val := Rbranch; Valid := V2|}); trivial.
+Qed.
+
+Lemma tree_itree_iso2_ {L A}
+  : cata to_itree \o rana fto_tree =e id (A:=itree L A).
+  rewrite cata_ana_hylo. Opaque hylo. simpl. intros x.
+  induction x as [l|n l Ihl r Ihr]; rewrite hylo_unr; simpl; trivial.
+  rewrite Ihl, Ihr. reflexivity.
+Qed.
+
+(* For some reason unfolding does not work ...? *)
+Lemma tree_itree_iso2 {L A}
+  : tree_to_itree \o itree_to_tree =e id (A:=itree L A).
+  exact tree_itree_iso2_.
+Qed.
 
 (* TODO: refactor into Utilities *)
 Lemma length_filter A (p : A -> bool) (l : list A) :
@@ -100,11 +162,6 @@ Proof.
       rewrite PeanoNat.Nat.lt_succ_r in LT.
       apply (PeanoNat.Nat.lt_le_trans _ _ _ LT' LT).
 Defined.
-
-Tactic Notation "|{" ident(x)  "~>" uconstr(T) "}|" :=
-  refine {| app := fun x => T |};
-  try (intros ??->; reflexivity);
-  try (let H := fresh "H" in intros ?? H; simpl in H; subst; reflexivity).
 
 Notation "'morph' T" :=
   (ltac:( T ))
